Move low_val lemmas to heap and make robust safety proof easier to read.

theories/heap_lang/robust_safety.v
@@ -8,163 +8,6 @@ Import uPred.
 
 Local Hint Resolve to_of_val.
 
-(** * Eliminating low values *)
-(**
-  These lemmas are useful at the boundary between verified and
-  adversarial code.
-*)
-Section wp_low_val.
-  Context `{heapG Σ}.
-  Implicit Types e : expr.
-  Implicit Types v : val.
-
-  Lemma wp_low_val_app v1 v2 :
-    {{{ low v1 ∗ low v2 }}} App (of_val v1) (of_val v2)
-    ?{{{ v, RET v; low v }}}.
-  Proof.
-    iIntros (Φ) "#[Hv1 Hv2] HΦ".
-    case: (decide (is_rec (of_val v1)))=>Hrec;
-      last by iApply wp_stuck_app_nrec.
-    move: Hrec=>[] f [] x [] erec Hrec.
-    case: (decide (Closed (f :b: x :b: []) erec))=>?;
-      last by iApply wp_stuck_app_open.
-    have->: v1 = RecV f x erec.
-    { apply (inj Some). by rewrite -to_val_rec Hrec to_of_val. }
-    rewrite (low_val (RecV _ _ _)) always_elim.
-    iApply wp_rec; [done|by exists v2|]. iNext.
-    iApply (wp_wand with "[] [$HΦ]"). by iApply ("Hv1" with "[$Hv2]").
-  Qed.
-
-  Lemma un_op_eval_low op v1 v2 : un_op_eval op v1 = Some v2 → low v2.
-  Proof.
-    by case: op; case: v1=> // -[] // ? /= [] <-; rewrite low_val low_lit.
-  Qed.
-
-  Lemma wp_low_val_un_op E op v Φ :
-    ▷(∀ v, low v -∗ Φ v) -∗ WP UnOp op (of_val v) @ E ?{{ Φ }}.
-  Proof.
-    iIntros "HΦ".
-    case EV: (un_op_eval op v)=>[v'|]; last by iApply wp_stuck_un_op.
-    wp_op. iApply "HΦ". by iApply un_op_eval_low.
-  Qed.
-
-  Lemma bin_op_eval_low op v1 v2 v3 :
-    bin_op_eval op v1 v2 = Some v3 → low v3.
-  Proof.
-    case: op; try by case: v1=> // -[] // ?; case: v2=>// -[] // ? /= [] <-;
-      rewrite low_val low_lit.
-    by rewrite/bin_op_eval; case: (bool_decide _)=> -[] <-;
-      rewrite low_val low_lit.
-  Qed.
-
-  Lemma wp_low_val_bin_op E op v1 v2 Φ :
-    ▷(∀ v, low v -∗ Φ v) -∗ WP BinOp op (of_val v1) (of_val v2) @ E ?{{ Φ }}.
-  Proof.
-    iIntros "HΦ".
-    case EV: (bin_op_eval op v1 v2)=>[v'|]; last by iApply wp_stuck_bin_op.
-    wp_op. iApply "HΦ". by iApply bin_op_eval_low.
-  Qed.
-
-  Lemma wp_low_val_if E v e1 e2 Φ :
-    ▷ (WP e1 @ E ?{{ Φ }} ∧ WP e2 @ E ?{{ Φ }}) -∗
-    WP If (of_val v) e1 e2 @ E ?{{ Φ }}.
-  Proof.
-    iIntros "Hes".
-    case: (decide (is_lit_bool (of_val v)))=>Hbool; last by iApply wp_stuck_if.
-    case: Hbool=>[] [] <-; wp_if.
-    by iDestruct "Hes" as "[? _]". by iDestruct "Hes" as "[_ ?]".
-  Qed.
-
-  Lemma wp_low_val_fst E v :
-    {{{ low v }}} Fst (of_val v) @ E ?{{{ v, RET v; low v }}}.
-  Proof.
-    iIntros (Φ) "#Hv HΦ".
-    case: (decide (is_pair_val (of_val v)))=>Hp; last by iApply wp_stuck_fst.
-    case: Hp=>e1 [] e2 [] [] v1 He1 [] [] v2 He2 Hp. rewrite Hp.
-    iApply wp_fst; [done|by exists v2|]. have->: v = PairV v1 v2.
-    { move: Hp He1 He2. case: v=> //= v1' v2' [] <-<-.
-      by rewrite 2!to_of_val => -[] -> [] ->. }
-    rewrite low_val. iDestruct "Hv" as "(Hv1&_)". iNext.
-    by iApply ("HΦ" with "[$Hv1]").
-  Qed.
-
-  Lemma wp_low_val_snd E v :
-    {{{ low v }}} Snd (of_val v) @ E ?{{{ v, RET v; low v }}}.
-  Proof.
-    iIntros (Φ) "#Hv HΦ".
-    case: (decide (is_pair_val (of_val v)))=>Hp; last by iApply wp_stuck_snd.
-    case: Hp=>e1 [] e2 [] [] v1 He1 [] [] v2 He2 Hp. rewrite Hp.
-    iApply wp_snd; [by exists v1|done|]. have->: v = PairV v1 v2.
-    { move: Hp He1 He2. case: v=> //= v1' v2' [] <-<-.
-      by rewrite 2!to_of_val => -[] -> [] ->. }
-    rewrite low_val. iDestruct "Hv" as "(_&Hv2)". iNext.
-    by iApply ("HΦ" with "[$Hv2]").
-  Qed.
-
-  Lemma wp_low_val_case E v e1 e2 Φ :
-    low v -∗
-    ▷ (∀ v0, low v0 -∗
-      WP App e1 (of_val v0) @ E ?{{ Φ }} ∧
-      WP App e2 (of_val v0) @ E ?{{ Φ }}) -∗
-    WP Case (of_val v) e1 e2 @ E ?{{ Φ }}.
-  Proof.
-    iIntros "#Hv Hk".
-    case: (decide (is_inj_val (of_val v)))=>Hc; last by iApply wp_stuck_case.
-    move: Hc=>[] e0 [] [] v0 He0 [] Hc; rewrite Hc -(of_to_val e0 v0) //.
-    - iApply wp_case_inl; first by exists v0.
-      have->: v = InjLV v0 by move: Hc He0; case: v => //= v' [] <-;
-        rewrite to_of_val => -[] ->.
-      rewrite low_val. iNext. setoid_rewrite and_elim_l.
-      by iApply ("Hk" with "[$Hv]").
-    - iApply wp_case_inr; first by exists v0.
-      have->: v = InjRV v0 by move: Hc He0; case: v => //= v' [] <-;
-        rewrite to_of_val => -[] ->.
-      rewrite low_val. iNext. setoid_rewrite and_elim_r.
-      by iApply ("Hk" with "[$Hv]").
-  Qed.
-
-  Lemma wp_low_val_load E v :
-    ↑heapN ⊆ E →
-    {{{ heap_ctx ∗ ▷low v }}} Load (of_val v) @ E ?{{{ v, RET v; low v }}}.
-  Proof.
-    iIntros (? Φ) "#(Hh&Hv) HΦ".
-    case: (decide (is_loc (of_val v)))=>Hl; last by iApply wp_stuck_load.
-    case: Hl=>l Hl. rewrite Hl.
-    iApply (wp_load_low with "[$Hh Hv] [$HΦ]"); first done.
-    have->: v = LitV (LitLoc l) by case: v Hl => // -[] //= ? [] ->.
-    rewrite low_val low_lit. by iFrame.
-  Qed.
-
-  Lemma wp_low_val_store E v1 v2 :
-    ↑heapN ⊆ E →
-    {{{ heap_ctx ∗ ▷low v1 ∗ ▷low v2 }}} Store (of_val v1) (of_val v2) @ E
-    ?{{{ v, RET v; low v }}}.
-  Proof.
-    iIntros (? Φ) "(Hh&Hv1&Hv2) HΦ".
-    case: (decide (is_loc (of_val v1)))=>Hl; last by iApply wp_stuck_store.
-    case: Hl=>l Hl. rewrite Hl.
-    iApply (wp_store_low with "[$Hh Hv1 $Hv2] [HΦ]"); [done|done| |].
-    - have->: v1 = LitV (LitLoc l) by case: v1 Hl => // -[] //= ? [] ->.
-      rewrite low_val low_lit. by iFrame.
-    - iNext. iIntros "_". iApply "HΦ". by rewrite low_val low_lit.
-  Qed.
-
-  Lemma wp_low_val_cas E v1 v2 v3 :
-    ↑heapN ⊆ E →
-    {{{ heap_ctx ∗ ▷low v1 ∗ ▷low v3 }}}
-      CAS (of_val v1) (of_val v2) (of_val v3) @ E
-    ?{{{ v, RET v; low v }}}.
-  Proof.
-    iIntros (? Φ) "(Hh&Hv1&Hv3) HΦ".
-    case: (decide (is_loc (of_val v1)))=>Hl; last by iApply wp_stuck_cas.
-    case: Hl=>l Hl. rewrite Hl.
-    iApply (wp_cas_low with "[$Hh Hv1 $Hv3] [HΦ]"); [done|done|done| |].
-    - have->: v1 = LitV (LitLoc l) by case: v1 Hl => // -[] //= ? [] ->.
-      rewrite low_val low_lit. by iFrame.
-    - iNext. iIntros (b) "_". iApply "HΦ". by rewrite low_val low_lit.
-  Qed.
-End wp_low_val.
-
 (** * Substitution of values for binders *)
 Section substitution.
   Context `{heapG Σ}.
@@ -189,13 +32,14 @@ Section substitution.
   |}.
 
   Definition env := gmap binder val.
-  Implicit Types Γ : env.
+  Implicit Types γ : env.
 
   Definition substitute_acc : binder * val → (expr → expr) → expr → expr :=
     λ xv f, let: (x, v) := xv in λ e, subst' x (of_val v) (f e).
   Definition substitute' : list (binder * val) → expr → expr :=
     foldr substitute_acc id.
   Definition substitute : env → expr → expr := substitute' ∘ map_to_list.
+  Coercion substitute : env >-> Funclass.
 
   Lemma substitute'_cons x v L e :
     substitute' ((x, v) :: L) e = subst' x (of_val v) (substitute' L e).
@@ -229,81 +73,80 @@ Section substitution.
       by eapply Hfun; eapply elem_of_list_permutation_proper.
   Qed.
 
-  Lemma substitute_empty e : e = substitute ∅ e. Proof. by []. Qed.
-
-  Lemma subst_substitute Γ x v e :
-    Γ !! x = None →
-    subst' x (of_val v) (substitute Γ e) = substitute (<[x:=v]>Γ) e.
+  Lemma subst_substitute γ x v e :
+    γ !! x = None → subst' x (of_val v) (γ e) = (<[x:=v]>γ) e.
   Proof.
     move=>?. rewrite /substitute/compose -substitute'_cons.
     symmetry. apply substitute'_proper.
     exact: map_to_list_unique. by rewrite map_to_list_insert.
   Qed.
 
-  Lemma substitute_closed Γ e : Closed [] e → substitute Γ e = e.
+  Lemma substitute_closed γ e : Closed [] e → γ e = e.
   Proof.
-    move=>?. induction Γ as [|x v Γ Hx IH] using map_ind; first done.
+    move=>?. induction γ as [|x v γ Hx IH] using map_ind; first done.
     rewrite -subst_substitute // IH.
     case: x Hx=> //= x Hx. exact: subst_is_closed_nil.
   Qed.
 
-  Lemma substitute_expr : ∀ Γ e, let s := substitute Γ in
-    s e =
+  Lemma substitute_empty e : (∅ : env) e = e. Proof. by []. Qed.
+
+  Lemma substitute_expr γ e :
+    γ e =
     match e with
-    | Var x => default (Var x) (Γ !! BNamed x) of_val
-    | Rec f x e => Rec f x $ substitute (delete f $ delete x $ Γ) e
-    | App e1 e2 => App (s e1) (s e2)
+    | Var x => default (Var x) (γ !! BNamed x) of_val
+    | Rec f x e => Rec f x $ (delete f $ delete x $ γ) e
+    | App e1 e2 => App (γ e1) (γ e2)
     | Lit lit => e
-    | UnOp op e => UnOp op (s e)
-    | BinOp op e1 e2 => BinOp op (s e1) (s e2)
-    | If e1 e2 e3 => If (s e1) (s e2) (s e3)
-    | Pair e1 e2 => Pair (s e1) (s e2)
-    | Fst e => Fst (s e)
-    | Snd e => Snd (s e)
-    | InjL e => InjL (s e)
-    | InjR e => InjR (s e)
-    | Case e1 e2 e3 => Case (s e1) (s e2) (s e3)
-    | Assert e => Assert (s e)
-    | Fork e => Fork (s e)
-    | Alloc e => Alloc (s e)
-    | Load e => Load (s e)
-    | Store e1 e2 => Store (s e1) (s e2)
-    | CAS e1 e2 e3 => CAS (s e1) (s e2) (s e3)
+    | UnOp op e => UnOp op (γ e)
+    | BinOp op e1 e2 => BinOp op (γ e1) (γ e2)
+    | If e1 e2 e3 => If (γ e1) (γ e2) (γ e3)
+    | Pair e1 e2 => Pair (γ e1) (γ e2)
+    | Fst e => Fst (γ e)
+    | Snd e => Snd (γ e)
+    | InjL e => InjL (γ e)
+    | InjR e => InjR (γ e)
+    | Case e1 e2 e3 => Case (γ e1) (γ e2) (γ e3)
+    | Assert e => Assert (γ e)
+    | Fork e => Fork (γ e)
+    | Alloc e => Alloc (γ e)
+    | Load e => Load (γ e)
+    | Store e1 e2 => Store (γ e1) (γ e2)
+    | CAS e1 e2 e3 => CAS (γ e1) (γ e2) (γ e3)
     end.
   Proof.
-    have nullary: ∀ Γ e, (∀ x es, subst x es e = e) → substitute Γ e = e.
-    { move=>Γ e Hf.
+    move: γ e.
+    have nullary: ∀ γ e, (∀ x es, subst x es e = e) → γ e = e.
+    { move=>γ e Hf.
       have{Hf} Hf: ∀ x es, subst' x es e = e by case.
-      induction Γ as [|x v Γ Hx IH] using map_ind; first done.
+      induction γ as [|x v γ Hx IH] using map_ind; first done.
       by rewrite -subst_substitute // IH Hf. }
-    Local Ltac by_induction Γ Hf :=
+    Local Ltac by_induction γ Hf :=
       let IH := fresh "IH" in
-      induction Γ as [|x v Γ Hx IH] using map_ind; first done;
+      induction γ as [|x v γ Hx IH] using map_ind; first done;
       by rewrite -subst_substitute // IH Hf; f_equal; rewrite subst_substitute.
-    have unary: ∀ f Γ e, (∀ x es e, subst x es (f e) = f (subst x es e)) →
-      substitute Γ (f e) = f (substitute Γ e).
-    { move=>f Γ e Hf.
+    have unary: ∀ f γ e, (∀ x es e, subst x es (f e) = f (subst x es e)) →
+      γ (f e) = f (γ e).
+    { move=>f γ e Hf.
       have{Hf} Hf: ∀ x es e, subst' x es (f e) = f (subst' x es e) by case.
-      by_induction Γ Hf. }
-    have binary: ∀ f Γ e1 e2,
+      by_induction γ Hf. }
+    have binary: ∀ f γ e1 e2,
       (∀ x es e1 e2, subst x es (f e1 e2) = f (subst x es e1) (subst x es e2)) →
-      substitute Γ (f e1 e2) = f (substitute Γ e1) (substitute Γ e2).
-    { move=>f Γ e1 e2 Hf.
+      substitute γ (f e1 e2) = f (substitute γ e1) (substitute γ e2).
+    { move=>f γ e1 e2 Hf.
       have{Hf} Hf: ∀ x es e1 e2, subst' x es (f e1 e2) =
          f (subst' x es e1) (subst' x es e2) by case.
-      by_induction Γ Hf. }
-    have ternary: ∀ f Γ e1 e2 e3,
+      by_induction γ Hf. }
+    have ternary: ∀ f γ e1 e2 e3,
       (∀ x es e1 e2 e3, subst x es (f e1 e2 e3) =
        f (subst x es e1) (subst x es e2) (subst x es e3)) →
-      substitute Γ (f e1 e2 e3) =
-      f (substitute Γ e1) (substitute Γ e2) (substitute Γ e3).
-    { move=>f Γ e1 e2 e3 Hf.
+      γ (f e1 e2 e3) = f (γ e1) (γ e2) (γ e3).
+    { move=>f γ e1 e2 e3 Hf.
       have{Hf} Hf: ∀ x es e1 e2 e3, subst' x es (f e1 e2 e3) =
         f (subst' x es e1) (subst' x es e2) (subst' x es e3) by case.
-      by_induction Γ Hf. }
-    move=>Γ /= []; try by auto using nullary, unary, binary, ternary.
+      by_induction γ Hf. }
+    move=>γ /= []; try by auto using nullary, unary, binary, ternary.
     - move=> x {nullary unary binary ternary}.
-      induction Γ as [|y v Γ Hy IH] using map_ind; first done.
+      induction γ as [|y v γ Hy IH] using map_ind; first done.
       rewrite -subst_substitute // IH {IH}. case: (decide (BNamed x = y)) => ?.
       { subst. by rewrite Hy lookup_insert /= /subst decide_True. }
       rewrite lookup_insert_ne //. destruct y as [|y]; first done.
@@ -311,7 +154,7 @@ Section substitution.
       + rewrite subst_is_closed_nil //. exact: is_closed_of_val.
       + rewrite/subst decide_False // => ?. by subst.
     - move=>f x e {nullary unary binary ternary}.
-      induction Γ as [|y v Γ Hy IH] using map_ind; first done.
+      induction γ as [|y v γ Hy IH] using map_ind; first done.
       rewrite -subst_substitute // IH {IH}.
       case: (decide (y ≠ f ∧ y ≠ x))=>[[??]| /not_and_l EQ].
       { rewrite subst_rec_ne'; [| by left | by left]. f_equal.
@@ -341,23 +184,23 @@ End substitution.
 Section ftlr.
 
   Context `{heapG Σ}.
-  Implicit Types Γ : env.
+  Implicit Types γ : env.
   Implicit Types e : expr.
   Implicit Types v : val.
 
-  Instance env_low : LowIntegrity Σ env := Low (λ Γ, [∗ map] v ∈ Γ, low v)%I _.
+  Instance env_low : LowIntegrity Σ env := Low (λ γ, [∗ map] v ∈ γ, low v)%I _.
 
   Definition confined : expr → iProp Σ := λ e, (
-    ∀ Γ, heap_ctx -∗ low Γ -∗ low e -∗ WP substitute Γ e ?{{ low }}
+    ∀ γ, heap_ctx -∗ low γ -∗ low e -∗ WP γ e ?{{ low }}
   )%I.
 
-  Lemma low_env Γ : low Γ ⊣⊢ [∗ map] v ∈ Γ, low v. Proof. by []. Qed.
+  Lemma low_env γ : low γ ⊣⊢ [∗ map] v ∈ γ, low v. Proof. by []. Qed.
 
   Lemma low_env_empty : low (∅ : env) ⊣⊢ True.
   Proof. exact: big_sepM_empty. Qed.
 
-  Lemma low_env_insert Γ x v :
-    Γ !! x = None → low v -∗ low Γ -∗ low (<[x:=v]>Γ).
+  Lemma low_env_insert γ x v :
+    γ !! x = None → low v -∗ low γ -∗ low (<[x:=v]>γ).
   Proof.
     do 2!rewrite low_env. move=>?. rewrite big_sepM_insert //.
     iIntros. by iFrame "#".
@@ -366,45 +209,46 @@ Section ftlr.
   Lemma low_env_singleton x v : low ({[x:=v]} : env) ⊣⊢ low v.
   Proof. exact: big_sepM_singleton. Qed.
 
-  Lemma low_env_lookup Γ x v : Γ !! x = Some v → low Γ -∗ low v.
+  Lemma low_env_lookup γ x v : γ !! x = Some v → low γ -∗ low v.
   Proof. exact: big_sepM_lookup. Qed.
 
-  Lemma low_env_delete Γ x  : low Γ -∗ low (delete x Γ).
+  Lemma low_env_delete γ x  : low γ -∗ low (delete x γ).
   Proof.
     rewrite low_env. apply big_sepM_mono. exact: delete_subseteq. done.
   Qed.
 
   Lemma confined_alt e :
     confined e ⊣⊢
-    ∀ Γ Φ, heap_ctx -∗ low Γ -∗ low e -∗ (∀ v, low v -∗ Φ v) -∗
-    WP substitute Γ e ?{{ Φ }}.
+    ∀ γ Φ, heap_ctx -∗ low γ -∗ low e -∗ (∀ v, low v -∗ Φ v) -∗
+    WP γ e ?{{ Φ }}.
   Proof.
     iSplit.
-    - iIntros "Hc". iIntros (Γ Φ) "Hh HΓ He". rewrite -wp_wand.
-      by iApply ("Hc" with "[$Hh] [$HΓ] [$He]").
-    - iIntros "Halt". iIntros (Γ) "Hh HΓ He".
-      iApply ("Halt" with "[$Hh] [$HΓ] [$He] []"). by iIntros.
+    - iIntros "Hc". iIntros (γ Φ) "Hh Hγ He". rewrite -wp_wand.
+      by iApply ("Hc" with "[$Hh] [$Hγ] [$He]").
+    - iIntros "Halt". iIntros (γ) "Hh Hγ He".
+      iApply ("Halt" with "[$Hh] [$Hγ] [$He] []"). by iIntros.
   Qed.
 
   Lemma confined_var x : confined (Var x).
   Proof.
-    iIntros (Γ) "_ #HΓ _". rewrite substitute_expr.
+    iIntros (γ) "_ #Hγ _". rewrite substitute_expr.
     case Hdom: (_ !! _)=>[v|]/=; last by iApply wp_stuck_var.
-    iApply wp_value'. by iApply (low_env_lookup with "[$HΓ]").
+    iApply wp_value'. by iApply (low_env_lookup with "[$Hγ]").
   Qed.
+  Hint Extern 1 (_ ⊢ confined (Var _)) => rewrite -confined_var.
 
   Lemma of_val_rec f x e `{!Closed (f :b: x :b: []) e} :
     Rec f x e = of_val (RecV f x e).
   Proof. symmetry. apply of_to_val. exact: to_val_rec. Qed.
 
-  Lemma confined_rec f x e : (□ confined e) -∗ confined (Rec f x e).
+  Lemma confined_rec f x e : □ confined e -∗ confined (Rec f x e).
   Proof.
-    iIntros "#IHe". iIntros (Γ) "#Hh #HΓ #He".
+    iIntros "#IHe". iIntros (γ) "#Hh #Hγ #He".
     rewrite low_expr substitute_expr. set erec := substitute _ _.
     case: (decide (Closed (f :b: x :b: []) erec)) => ?;
       last by iApply wp_stuck_rec_open.
     iApply wp_value; first exact: to_val_rec.
-    rewrite/erec. set Γ' := (delete _ _).
+    rewrite/erec. set γ' := (delete _ _).
     iLöb as "Hvrec". rewrite {2}low_val. iAlways. iNext.
     iIntros (v2) "#Hv2". case: (decide (x = f))=>?.
     { subst. rewrite -> subst_subst'; last done.	(* ssr rewrite fails *)
@@ -412,7 +256,7 @@ Section ftlr.
       iApply ("IHe" with "[$Hh] [] [$He]").
       rewrite insert_delete. iApply (low_env_insert with "[$Hvrec] []");
         first by rewrite lookup_delete.
-      by iApply (low_env_delete with "[$HΓ]"). }
+      by iApply (low_env_delete with "[$Hγ]"). }
     rewrite of_val_rec subst_substitute; last by rewrite lookup_delete.
     rewrite subst_substitute; last by rewrite
       lookup_insert_ne // lookup_delete_ne // lookup_delete.
@@ -421,230 +265,243 @@ Section ftlr.
       lookup_insert_ne // lookup_delete_ne // lookup_delete.
     iApply (low_env_insert with "[$Hvrec] []"); first by rewrite
       lookup_delete.
-    do 2!iApply low_env_delete. iExact "HΓ".
+    do 2!iApply low_env_delete. iExact "Hγ".
   Qed.
+  Hint Extern 1 (_ ⊢ confined (Rec _ _ _))
+    => rewrite -confined_rec; exact: always_intro.
 
-  Lemma confined_app e1 e2 : confined e1 -∗ confined e2 -∗ confined (App e1 e2).
+  Lemma confined_app e1 e2 : confined e1 ∗ confined e2 -∗ confined (App e1 e2).
   Proof.
     rewrite (confined_alt (App _ _)).
-    iIntros "IHe1 IHe2". iIntros (Γ Φ) "#Hh #HΓ Happ HΦ".
+    iIntros "[IHe1 IHe2]". iIntros (γ Φ) "#Hh #Hγ Happ HΦ".
     rewrite low_expr substitute_expr. iDestruct "Happ" as "(He1&He2)".
-    wp_bind (substitute _ _). rewrite confined_alt.
-    iApply ("IHe1" with "[$Hh] [$HΓ] [$He1]"). iIntros (v1) "Hv1".
-    wp_bind (substitute _ _). rewrite confined_alt.
-    iApply ("IHe2" with "[$Hh] [$HΓ] [$He2]"). iIntros (v2) "Hv2".
+    wp_bind (γ _). rewrite confined_alt.
+    iApply ("IHe1" with "[$Hh] [$Hγ] [$He1]"). iIntros (v1) "Hv1".
+    wp_bind (γ _). rewrite confined_alt.
+    iApply ("IHe2" with "[$Hh] [$Hγ] [$He2]"). iIntros (v2) "Hv2".
     by iApply (wp_low_val_app with "[$Hv1 $Hv2] [$HΦ]").
   Qed.
+  Hint Extern 1 (_ ⊢ confined (App _ _)) => rewrite -confined_app.
 
   Lemma confined_lit lit : confined (Lit lit).
   Proof.
-    iIntros (Γ) "_ _ #?". rewrite low_expr substitute_expr.
+    iIntros (γ) "_ _ #?". rewrite low_expr substitute_expr.
     iApply wp_value; first done. by rewrite low_val.
   Qed.
+  Hint Extern 1 (_ ⊢ confined (Lit _)) => rewrite -confined_lit.
 
   Lemma confined_un_op op e : confined e -∗ confined (UnOp op e).
   Proof.
     rewrite (confined_alt (UnOp _ _)).
-    iIntros "IHe". iIntros (Γ Φ) "Hh HΓ He HΦ".
+    iIntros "IHe". iIntros (γ Φ) "Hh Hγ He HΦ".
     rewrite low_expr substitute_expr.
-    wp_bind (substitute _ _). rewrite confined_alt.
-    iApply ("IHe" with "[$Hh] [$HΓ] [$He]"). iIntros (v) "_".
+    wp_bind (γ _). rewrite confined_alt.
+    iApply ("IHe" with "[$Hh] [$Hγ] [$He]"). iIntros (v) "_".
     by iApply (wp_low_val_un_op with "[$HΦ]").
   Qed.
+  Hint Extern 1 (_ ⊢ confined (UnOp _ _)) => rewrite -confined_un_op.
 
   Lemma confined_bin_op op e1 e2 :
-    confined e1 -∗ confined e2 -∗ confined (BinOp op e1 e2).
+    confined e1 ∗ confined e2 -∗ confined (BinOp op e1 e2).
   Proof.
     rewrite (confined_alt (BinOp _ _ _)).
-    iIntros "IHe1 IHe2". iIntros (Γ Φ) "#Hh #HΓ Hop HΦ".
+    iIntros "[IHe1 IHe2]". iIntros (γ Φ) "#Hh #Hγ Hop HΦ".
     rewrite low_expr substitute_expr. iDestruct "Hop" as "(He1&He2)".
-    wp_bind (substitute _ _). rewrite confined_alt.
-    iApply ("IHe1" with "[$Hh] [$HΓ] [$He1]"). iIntros (v1) "_".
-    wp_bind (substitute _ _). rewrite confined_alt.
-    iApply ("IHe2" with "[$Hh] [$HΓ] [$He2]"). iIntros (v2) "_".
+    wp_bind (γ _). rewrite confined_alt.
+    iApply ("IHe1" with "[$Hh] [$Hγ] [$He1]"). iIntros (v1) "_".
+    wp_bind (γ _). rewrite confined_alt.
+    iApply ("IHe2" with "[$Hh] [$Hγ] [$He2]"). iIntros (v2) "_".
     by iApply (wp_low_val_bin_op with "[$HΦ]").
   Qed.
+  Hint Extern 1 (_ ⊢ confined (BinOp _ _ _)) => rewrite -confined_bin_op.
 
   Lemma confined_if e e1 e2 :
-    confined e -∗ confined e1 -∗ confined e2 -∗ confined (If e e1 e2).
+    confined e ∗ confined e1 ∗ confined e2 -∗ confined (If e e1 e2).
   Proof.
     rewrite (confined_alt (If _ _ _)).
-    iIntros "IHe IHe1 IHe2". iIntros (Γ Φ) "#Hh #HΓ Hif HΦ".
+    iIntros "(IHe&IHe1&IHe2)". iIntros (γ Φ) "#Hh #Hγ Hif HΦ".
     rewrite low_expr substitute_expr. iDestruct "Hif" as "(He&He1&He2)".
-    wp_bind (substitute _ _). rewrite confined_alt.
-    iApply ("IHe" with "[$Hh] [$HΓ] [$He]"). iIntros (v) "_".
+    wp_bind (γ _). rewrite confined_alt.
+    iApply ("IHe" with "[$Hh] [$Hγ] [$He]"). iIntros (v) "_".
     iApply wp_low_val_if. iNext. iSplit.
     - rewrite confined_alt.
-      by iApply ("IHe1" with "[$Hh] [$HΓ] [$He1] [$HΦ]").
+      by iApply ("IHe1" with "[$Hh] [$Hγ] [$He1] [$HΦ]").
     - rewrite (confined_alt e2).
-      by iApply ("IHe2" with "[$Hh] [$HΓ] [$He2] [$HΦ]").
+      by iApply ("IHe2" with "[$Hh] [$Hγ] [$He2] [$HΦ]").
   Qed.
+  Hint Extern 1 (_ ⊢ confined (If _ _ _)) => rewrite -confined_if.
 
   Lemma confined_pair e1 e2 :
-    confined e1 -∗ confined e2 -∗ confined (Pair e1 e2).
+    confined e1 ∗ confined e2 -∗ confined (Pair e1 e2).
   Proof.
     rewrite (confined_alt (Pair _ _)).
-    iIntros "IHe1 IHe2". iIntros (Γ Φ) "#Hh #HΓ Hp HΦ".
+    iIntros "[IHe1 IHe2]". iIntros (γ Φ) "#Hh #Hγ Hp HΦ".
     rewrite low_expr substitute_expr. iDestruct "Hp" as "(He1&He2)".
-    wp_bind (substitute _ _). rewrite confined_alt.
-    iApply ("IHe1" with "[$Hh] [$HΓ] [$He1]"). iIntros (v1) "Hv1".
-    wp_bind (substitute _ _). rewrite confined_alt.
-    iApply ("IHe2" with "[$Hh] [$HΓ] [$He2]"). iIntros (v2) "Hv2".
+    wp_bind (γ _). rewrite confined_alt.
+    iApply ("IHe1" with "[$Hh] [$Hγ] [$He1]"). iIntros (v1) "Hv1".
+    wp_bind (γ _). rewrite confined_alt.
+    iApply ("IHe2" with "[$Hh] [$Hγ] [$He2]"). iIntros (v2) "Hv2".
     iApply wp_value; first by rewrite /= (to_of_val v1) (to_of_val v2).
     iApply "HΦ". rewrite (low_val (PairV _ _)). by iFrame.
   Qed.
+  Hint Extern 1 (_ ⊢ confined (Pair _ _)) => rewrite -confined_pair.
 
   Lemma confined_fst e : confined e -∗ confined (Fst e).
   Proof.
     rewrite (confined_alt (Fst _)).
-    iIntros "IHe". iIntros (Γ Φ) "#Hh #HΓ He HΦ".
+    iIntros "IHe". iIntros (γ Φ) "#Hh #Hγ He HΦ".
     rewrite low_expr substitute_expr.
-    wp_bind (substitute _ _). rewrite confined_alt.
-    iApply ("IHe" with "[$Hh] [$HΓ] [$He]"). iIntros (v) "Hv".
+    wp_bind (γ _). rewrite confined_alt.
+    iApply ("IHe" with "[$Hh] [$Hγ] [$He]"). iIntros (v) "Hv".
     by iApply (wp_low_val_fst with "[$Hv] [$HΦ]").
   Qed.
+  Hint Extern 1 (_ ⊢ confined (Fst _)) => rewrite -confined_fst.
 
   Lemma confined_snd e : confined e -∗ confined (Snd e).
   Proof.
     rewrite (confined_alt (Snd _)).
-    iIntros "IHe". iIntros (Γ Φ) "#Hh #HΓ He HΦ".
+    iIntros "IHe". iIntros (γ Φ) "#Hh #Hγ He HΦ".
     rewrite low_expr substitute_expr.
-    wp_bind (substitute _ _). rewrite confined_alt.
-    iApply ("IHe" with "[$Hh] [$HΓ] [$He]"). iIntros (v) "Hv".
+    wp_bind (γ _). rewrite confined_alt.
+    iApply ("IHe" with "[$Hh] [$Hγ] [$He]"). iIntros (v) "Hv".
     by iApply (wp_low_val_snd with "[$Hv] [$HΦ]").
   Qed.
+  Hint Extern 1 (_ ⊢ confined (Snd _)) => rewrite -confined_snd.
 
   Lemma confined_inl e : confined e -∗ confined (InjL e).
   Proof.
     rewrite (confined_alt (InjL _)).
-    iIntros "IHe". iIntros (Γ Φ) "#Hh #HΓ He HΦ".
+    iIntros "IHe". iIntros (γ Φ) "#Hh #Hγ He HΦ".
     rewrite low_expr substitute_expr.
-    wp_bind (substitute _ _). rewrite confined_alt.
-    iApply ("IHe" with "[$Hh] [$HΓ] [$He]"). iIntros (v) "Hv".
+    wp_bind (γ _). rewrite confined_alt.
+    iApply ("IHe" with "[$Hh] [$Hγ] [$He]"). iIntros (v) "Hv".
     iApply wp_value; first by rewrite /= (to_of_val v).
     iApply "HΦ". rewrite (low_val (InjLV _)). by iFrame.
   Qed.
+  Hint Extern 1 (_ ⊢ confined (InjL _)) => rewrite -confined_inl.
 
   Lemma confined_inr e : confined e -∗ confined (InjR e).
   Proof.
     rewrite (confined_alt (InjR _)).
-    iIntros "IHe". iIntros (Γ Φ) "#Hh #HΓ He HΦ".
+    iIntros "IHe". iIntros (γ Φ) "#Hh #Hγ He HΦ".
     rewrite low_expr substitute_expr.
-    wp_bind (substitute _ _). rewrite confined_alt.
-    iApply ("IHe" with "[$Hh] [$HΓ] [$He]"). iIntros (v) "Hv".
+    wp_bind (γ _). rewrite confined_alt.
+    iApply ("IHe" with "[$Hh] [$Hγ] [$He]"). iIntros (v) "Hv".
     iApply wp_value; first by rewrite /= (to_of_val v).
     iApply "HΦ". rewrite (low_val (InjRV _)). by iFrame.
   Qed.
+  Hint Extern 1 (_ ⊢ confined (InjR _)) => rewrite -confined_inr.
 
   Lemma confined_case e e1 e2 :
-    confined e -∗ confined e1 -∗ confined e2 -∗ confined (Case e e1 e2).
+    confined e ∗ confined e1 ∗ confined e2 -∗ confined (Case e e1 e2).
   Proof.
     rewrite (confined_alt (Case _ _ _)).
-    iIntros "IHe IHe1 IHe2". iIntros (Γ Φ) "#Hh #HΓ Hc HΦ".
+    iIntros "(IHe&IHe1&IHe2)". iIntros (γ Φ) "#Hh #Hγ Hc HΦ".
     rewrite low_expr substitute_expr. iDestruct "Hc" as "(He&He1&He2)".
-    wp_bind (substitute _ _). rewrite confined_alt.
-    iApply ("IHe" with "[$Hh] [$HΓ] [$He]"). iIntros (v) "Hv".
+    wp_bind (γ _). rewrite confined_alt.
+    iApply ("IHe" with "[$Hh] [$Hγ] [$He]"). iIntros (v) "Hv".
     iApply (wp_low_val_case with "[$Hv]"). iNext. iIntros (v0) "#Hv0". iSplit.
-    - wp_bind (substitute _ _). rewrite confined_alt.
-      iApply ("IHe1" with "[$Hh] [$HΓ] [$He1]"). iIntros (v1) "Hv1".
+    - wp_bind (γ _). rewrite confined_alt.
+      iApply ("IHe1" with "[$Hh] [$Hγ] [$He1]"). iIntros (v1) "Hv1".
       by iApply (wp_low_val_app with "[$Hv1 $Hv0] [$HΦ]").
-    - wp_bind (substitute _ _). rewrite (confined_alt e2).
-      iApply ("IHe2" with "[$Hh] [$HΓ] [$He2]"). iIntros (v2) "Hv2".
+    - wp_bind (γ _). rewrite (confined_alt e2).
+      iApply ("IHe2" with "[$Hh] [$Hγ] [$He2]"). iIntros (v2) "Hv2".
       by iApply (wp_low_val_app with "[$Hv2 $Hv0] [$HΦ]").
   Qed.
+  Hint Extern 1 (_ ⊢ confined (Case _ _ _)) => rewrite -confined_case.
 
   Lemma confined_assert e : confined (Assert e).
-  Proof. iIntros (Γ) "_ _ He". rewrite low_expr. by iExFalso. Qed.
+  Proof. iIntros (γ) "_ _ He". rewrite low_expr. by iExFalso. Qed.
+  Hint Extern 1 (_ ⊢ confined (Assert _)) => rewrite -confined_assert.
 
   Lemma confined_fork e : confined e -∗ confined (Fork e).
   Proof.
-    iIntros "IHe". iIntros (Γ) "#Hh #HΓ He".
+    iIntros "IHe". iIntros (γ) "#Hh #Hγ He".
     rewrite low_expr substitute_expr. iApply wp_fork. iNext. iSplit.
     - by rewrite low_val low_lit.
     - rewrite confined_alt.
-      iApply ("IHe" with "[$Hh] [$HΓ] [$He] []"). by iIntros.
+      iApply ("IHe" with "[$Hh] [$Hγ] [$He] []"). by iIntros.
   Qed.
+  Hint Extern 1 (_ ⊢ confined (Fork _)) => rewrite -confined_fork.
 
   Lemma confined_alloc e : confined e -∗ confined (Alloc e).
   Proof.
     rewrite (confined_alt (Alloc _)).
-    iIntros "IHe". iIntros (Γ Φ) "#Hh #HΓ He HΦ".
+    iIntros "IHe". iIntros (γ Φ) "#Hh #Hγ He HΦ".
     rewrite low_expr substitute_expr.
-    wp_bind (substitute _ _). rewrite confined_alt.
-    iApply ("IHe" with "[$Hh] [$HΓ] [$He]"). iIntros (v) "Hv".
+    wp_bind (γ _). rewrite confined_alt.
+    iApply ("IHe" with "[$Hh] [$Hγ] [$He]"). iIntros (v) "Hv".
     iApply (wp_alloc_low with "[$Hh $Hv]"); [by rewrite to_of_val|done|].
     iNext. iIntros (l) "#Hl". iApply "HΦ". by rewrite low_val low_lit.
   Qed.
+  Hint Extern 1 (_ ⊢ confined (Alloc _)) => rewrite -confined_alloc.
 
   Lemma confined_load e : confined e -∗ confined (Load e).
   Proof.
     rewrite (confined_alt (Load _)).
-    iIntros "IHe". iIntros (Γ Φ) "#Hh #HΓ He HΦ".
+    iIntros "IHe". iIntros (γ Φ) "#Hh #Hγ He HΦ".
     rewrite low_expr substitute_expr.
-    wp_bind (substitute _ _). rewrite confined_alt.
-    iApply ("IHe" with "[$Hh] [$HΓ] [$He]"). iIntros (v) "Hv".
+    wp_bind (γ _). rewrite confined_alt.
+    iApply ("IHe" with "[$Hh] [$Hγ] [$He]"). iIntros (v) "Hv".
     by iApply (wp_low_val_load with "[$Hh $Hv] [$HΦ]").
   Qed.
+  Hint Extern 1 (_ ⊢ confined (Load _)) => rewrite -confined_load.
 
   Lemma confined_store e1 e2 :
-    confined e1 -∗ confined e2 -∗ confined (Store e1 e2).
+    confined e1 ∗ confined e2 -∗ confined (Store e1 e2).
   Proof.
     rewrite (confined_alt (Store _ _)).
-    iIntros "IHe1 IHe2". iIntros (Γ Φ) "#Hh #HΓ Hstore HΦ".
+    iIntros "[IHe1 IHe2]". iIntros (γ Φ) "#Hh #Hγ Hstore HΦ".
     rewrite low_expr substitute_expr. iDestruct "Hstore" as "(He1&He2)".
-    wp_bind (substitute _ _). rewrite confined_alt.
-    iApply ("IHe1" with "[$Hh] [$HΓ] [$He1]"). iIntros (v1) "Hv1".
-    wp_bind (substitute _ _). rewrite confined_alt.
-    iApply ("IHe2" with "[$Hh] [$HΓ] [$He2]"). iIntros (v2) "Hv2".
+    wp_bind (γ _). rewrite confined_alt.
+    iApply ("IHe1" with "[$Hh] [$Hγ] [$He1]"). iIntros (v1) "Hv1".
+    wp_bind (γ _). rewrite confined_alt.
+    iApply ("IHe2" with "[$Hh] [$Hγ] [$He2]"). iIntros (v2) "Hv2".
     by iApply (wp_low_val_store with "[$Hh $Hv1 $Hv2] [$HΦ]").
   Qed.
+  Hint Extern 1 (_ ⊢ confined (Store _ _)) => rewrite -confined_store.
 
   Lemma confined_cas e0 e1 e2 :
-    confined e0 -∗ confined e1 -∗ confined e2 -∗ confined (CAS e0 e1 e2).
+    confined e0 ∗ confined e1 ∗ confined e2 -∗ confined (CAS e0 e1 e2).
   Proof.
     rewrite (confined_alt (CAS _ _ _)).
-    iIntros "IHe0 IHe1 IHe2". iIntros (Γ Φ) "#Hh #HΓ Hcas HΦ".
+    iIntros "(IHe0&IHe1&IHe2)". iIntros (γ Φ) "#Hh #Hγ Hcas HΦ".
     rewrite low_expr substitute_expr. iDestruct "Hcas" as "(He0&He1&He2)".
-    wp_bind (substitute _ _). rewrite confined_alt.
-    iApply ("IHe0" with "[$Hh] [$HΓ] [$He0]"). iIntros (v0) "Hv0".
-    wp_bind (substitute _ _). rewrite confined_alt.
-    iApply ("IHe1" with "[$Hh] [$HΓ] [$He1]"). iIntros (v1) "_".
-    wp_bind (substitute _ _). rewrite confined_alt.
-    iApply ("IHe2" with "[$Hh] [$HΓ] [$He2]"). iIntros (v2) "Hv2".
+    wp_bind (γ _). rewrite confined_alt.
+    iApply ("IHe0" with "[$Hh] [$Hγ] [$He0]"). iIntros (v0) "Hv0".
+    wp_bind (γ _). rewrite confined_alt.
+    iApply ("IHe1" with "[$Hh] [$Hγ] [$He1]"). iIntros (v1) "_".
+    wp_bind (γ _). rewrite confined_alt.
+    iApply ("IHe2" with "[$Hh] [$Hγ] [$He2]"). iIntros (v2) "Hv2".
     by iApply (wp_low_val_cas with "[$Hh $Hv0 $Hv2] [$HΦ]").
   Qed.
+  Hint Extern 1 (_ ⊢ confined (CAS _ _ _)) => rewrite -confined_cas.
+
+  Hint Extern 2 =>
+    match goal with
+    | IH : True ⊢ confined ?e |- True ⊢ confined (_ ?e) => rewrite IH
+    end.
+  Hint Extern 2 =>
+    match goal with
+    | IH1 : True ⊢ confined ?e1, IH2 : True ⊢ confined ?e2
+      |- True ⊢ confined (_ ?e1 ?e2)
+      => rewrite (True_sep_1 True) {1}IH1 IH2
+    end.
+  Hint Extern 2 =>
+    match goal with
+    | IH1 : True ⊢ confined ?e1, IH2 : True ⊢ confined ?e2,
+      IH3 : True ⊢ confined ?e3 |- True ⊢ confined (_ ?e1 ?e2 ?e3)
+      => rewrite (True_sep_1 True) {2}(True_sep_1 True) {1}IH1 {1}IH2 IH3
+    end.
 
   Theorem ftlr' e : confined e.
-  Proof.
-    iStartProof. (* iLöb as "IH" forall (e). *)
-    iInduction e as [| | | | | | | | | | | | | | | | | |] "IHe".
-    - by rewrite -confined_var.
-    - by rewrite -confined_rec.
-    - by iRevert "IHe1"; rewrite always_elim -confined_app.
-    - by rewrite -confined_lit.
-    - by rewrite -confined_un_op.
-    - by iRevert "IHe1"; rewrite always_elim -confined_bin_op.
-    - by iRevert "IHe1 IHe2"; rewrite 2!always_elim -confined_if.
-    - by iRevert "IHe1"; rewrite always_elim -confined_pair.
-    - by rewrite -confined_fst.
-    - by rewrite -confined_snd.
-    - by rewrite -confined_inl.
-    - by rewrite -confined_inr.
-    - by iRevert "IHe1 IHe2"; rewrite 2!always_elim -confined_case.
-    - by rewrite -confined_assert.
-    - by rewrite -confined_fork.
-    - by rewrite -confined_alloc.
-    - by rewrite -confined_load.
-    - by iRevert "IHe1"; rewrite always_elim -confined_store.
-    - by iRevert "IHe1 IHe2"; rewrite 2!always_elim -confined_cas.
-  Qed.
+  Proof. rewrite/uPred_valid. by induction e; auto. Qed.
 
-  Corollary ftlr e Γ e' Φ :
-    e = substitute Γ e' →
-    heap_ctx -∗ low Γ -∗ low e' -∗ (∀ v, low v -∗ Φ v) -∗ WP e ?{{ Φ }}.
+  Corollary ftlr γ e Φ :
+    heap_ctx -∗ low γ -∗ low e -∗ (∀ v, low v -∗ Φ v) -∗ WP γ e ?{{ Φ }}.
   Proof.
-    iIntros (->) "Hh HΓ He". rewrite -wp_wand.
-    iApply (ftlr' with "[$Hh] [$HΓ] [$He]").
+    iIntros "Hh Hγ He". rewrite -wp_wand.
+    by iApply (ftlr' with "[$Hh] [$Hγ] [$He]").
   Qed.
 End ftlr.
 
@@ -996,6 +853,7 @@ End adversary.
 Section robust_safety.
 
   Context `{heapG Σ}.
+  Implicit Types γ : env.
   Implicit Types C : ctx.
   Implicit Types e : expr.
   Implicit Types v : val.
@@ -1006,8 +864,8 @@ Section robust_safety.
   )%I.
 
   Definition safe : ctx → iProp Σ := λ C, (
-    ∀ Γ p e, heap_ctx -∗ low C -∗ low Γ -∗ □ verified p e -∗
-    WP substitute Γ (ctx_fill C e) ?{{ low }}
+    ∀ γ p e, heap_ctx -∗ low C -∗ low γ -∗ □ verified p e -∗
+    WP γ (ctx_fill C e) ?{{ low }}
   )%I.
 
   Lemma verified_alt p e :
@@ -1021,399 +879,402 @@ Section robust_safety.
 
   Lemma safe_alt C :
     safe C ⊣⊢
-    ∀ Γ p e Φ, heap_ctx -∗ low C -∗ low Γ -∗ □ verified p e -∗
-    (∀ v, low v -∗ Φ v) -∗ WP substitute Γ (ctx_fill C e) ?{{ Φ }}.
+    ∀ γ p e Φ, heap_ctx -∗ low C -∗ low γ -∗ □ verified p e -∗
+    (∀ v, low v -∗ Φ v) -∗ WP γ (ctx_fill C e) ?{{ Φ }}.
   Proof.
     iSplit.
-    - iIntros "Hsafe". iIntros (Γ p e Φ) "Hh HC HΓ He".
-      rewrite -wp_wand. by iApply ("Hsafe" with "[$Hh] [$HC] [$HΓ] [$He]").
-    - iIntros "Halt". iIntros (Γ p e) "Hh HC HΓ He".
-      iApply ("Halt" with "[$Hh] [$HC] [$HΓ] [$He] []"). by iIntros.
+    - iIntros "Hsafe". iIntros (γ p e Φ) "Hh HC Hγ He".
+      rewrite -wp_wand. by iApply ("Hsafe" with "[$Hh] [$HC] [$Hγ] [$He]").
+    - iIntros "Halt". iIntros (γ p e) "Hh HC Hγ He".
+      iApply ("Halt" with "[$Hh] [$HC] [$Hγ] [$He] []"). by iIntros.
   Qed.
 
   Lemma safe_hole : safe CHole.
   Proof.
-    iIntros (Γ p e) "_ _ _ >(%&He) /=". iApply (wp_forget_progress p).
+    iIntros (γ p e) "_ _ _ >(%&He) /=". iApply (wp_forget_progress p).
     by rewrite substitute_closed.
   Qed.
+  Hint Extern 1 (_ ⊢ safe CHole) => rewrite -safe_hole.
 
   Lemma safe_rec f x C : □ safe C -∗ safe (CRec f x C).
   Proof.
     (* PDS: Lots of duplication with confined_rec. *)
-    iIntros "#IH". iIntros (Γ p e) "#Hh #HC #HΓ #He /=".
+    iIntros "#IH". iIntros (γ p e) "#Hh #HC #Hγ #He /=".
     rewrite low_ctx substitute_expr. set erec := substitute _ _.
     case: (decide (Closed (f :b: x :b: []) erec)) => ?;
       last by iApply wp_stuck_rec_open.
     iApply wp_value; first exact: to_val_rec.
-    rewrite/erec. set Γ' := (delete _ _).
+    rewrite/erec. set γ' := (delete _ _).
     iLöb as "Hvrec". rewrite {2}low_val. iAlways. iNext.
     iIntros (v2) "#Hv2". case: (decide (x = f))=>?.
     { subst. rewrite -> subst_subst'; last done.	(* ssr rewrite fails *)
       rewrite of_val_rec subst_substitute; last by rewrite lookup_delete.
-      iApply ("IH" with "* [$Hh] [$HC] [] [He]"); last iExact "He". (* iNext bug *)
+      iApply ("IH" with "[$Hh] [$HC] [] [He]"); last iExact "He". (* iNext bug *)
       rewrite insert_delete. iApply (low_env_insert with "[$Hvrec] []");
         first by rewrite lookup_delete.
-      by iApply (low_env_delete with "[$HΓ]"). }
+      by iApply (low_env_delete with "[$Hγ]"). }
     rewrite of_val_rec subst_substitute; last by rewrite lookup_delete.
     rewrite subst_substitute; last by rewrite
       lookup_insert_ne // lookup_delete_ne // lookup_delete.
-    iApply ("IH" with "* [$Hh] [$HC] [] [He]"); last iExact "He". (* iNext bug *)
+    iApply ("IH" with "[$Hh] [$HC] [] [He]"); last iExact "He". (* iNext bug *)
     iApply (low_env_insert with "[$Hv2] []"); first by rewrite
       lookup_insert_ne // lookup_delete_ne // lookup_delete.
     iApply (low_env_insert with "[$Hvrec] []"); first by rewrite
       lookup_delete.
-    do 2!iApply low_env_delete. iExact "HΓ".
+    do 2!iApply low_env_delete. iExact "Hγ".
   Qed.
+  Hint Extern 1 (_ ⊢ safe (CRec _ _ _))
+    => rewrite -safe_rec; exact: always_intro.
 
   Lemma safe_app_l C1 e2 : safe C1 -∗ safe (CAppL C1 e2).
   Proof.
     rewrite (safe_alt (CAppL _ _)).
-    iIntros "IH". iIntros (Γ p e Φ) "#Hh Happ #HΓ He HΦ /=".
+    iIntros "IH". iIntros (γ p e Φ) "#Hh Happ #Hγ He HΦ /=".
     rewrite low_ctx substitute_expr. iDestruct "Happ" as "(HC1&He2)".
-    wp_bind (substitute _ _). rewrite safe_alt.
-    iApply ("IH" with "[$Hh] [$HC1] [$HΓ] [$He]"). iIntros (v1) "Hv1".
-    wp_bind (substitute _ _).
-    iApply (ftlr with "[$Hh] [$HΓ] [$He2]"); first done. iIntros (v2) "Hv2".
+    wp_bind (γ _). rewrite safe_alt.
+    iApply ("IH" with "[$Hh] [$HC1] [$Hγ] [$He]"). iIntros (v1) "Hv1".
+    wp_bind (γ _).
+    iApply (ftlr with "[$Hh] [$Hγ] [$He2]"). iIntros (v2) "Hv2".
     by iApply (wp_low_val_app with "[$Hv1 $Hv2] [$HΦ]").
   Qed.
+  Hint Extern 1 (_ ⊢ safe (CAppL _ _)) => rewrite -safe_app_l.
 
   Lemma safe_app_r e1 C2 : safe C2 -∗ safe (CAppR e1 C2).
   Proof.
     rewrite (safe_alt (CAppR _ _)).
-    iIntros "IH". iIntros (Γ p e Φ) "#Hh Happ #HΓ He HΦ /=".
+    iIntros "IH". iIntros (γ p e Φ) "#Hh Happ #Hγ He HΦ /=".
     rewrite low_ctx substitute_expr. iDestruct "Happ" as "(He1&HC2)".
-    wp_bind (substitute _ _).
-    iApply (ftlr with "[$Hh] [$HΓ] [$He1]"); first done. iIntros (v1) "Hv1".
-    wp_bind (substitute _ _). rewrite safe_alt.
-    iApply ("IH" with "[$Hh] [$HC2] [$HΓ] [$He]"). iIntros (v2) "Hv2".
+    wp_bind (γ _).
+    iApply (ftlr with "[$Hh] [$Hγ] [$He1]"). iIntros (v1) "Hv1".
+    wp_bind (γ _). rewrite safe_alt.
+    iApply ("IH" with "[$Hh] [$HC2] [$Hγ] [$He]"). iIntros (v2) "Hv2".
     by iApply (wp_low_val_app with "[$Hv1 $Hv2] [$HΦ]").
   Qed.
+  Hint Extern 1 (_ ⊢ safe (CAppR _ _)) => rewrite -safe_app_r.
 
   Lemma safe_un_op op C : safe C -∗ safe (CUnOp op C).
   Proof.
     rewrite (safe_alt (CUnOp _ _)).
-    iIntros "IH". iIntros (Γ p e Φ) "#Hh HC #HΓ He HΦ /=".
+    iIntros "IH". iIntros (γ p e Φ) "#Hh HC #Hγ He HΦ /=".
     rewrite low_ctx substitute_expr.
-    wp_bind (substitute _ _). rewrite safe_alt.
-    iApply ("IH" with "[$Hh] [$HC] [$HΓ] [$He]"). iIntros (v) "_".
+    wp_bind (γ _). rewrite safe_alt.
+    iApply ("IH" with "[$Hh] [$HC] [$Hγ] [$He]"). iIntros (v) "_".
     by iApply (wp_low_val_un_op with "[$HΦ]").
   Qed.
+  Hint Extern 1 (_ ⊢ safe (CUnOp _ _)) => rewrite -safe_un_op.
 
   Lemma safe_bin_op_l op C1 e2 : safe C1 -∗ safe (CBinOpL op C1 e2).
   Proof.
     rewrite (safe_alt (CBinOpL _ _ _)).
-    iIntros "IH". iIntros (Γ p e Φ) "#Hh Hop #HΓ He HΦ /=".
+    iIntros "IH". iIntros (γ p e Φ) "#Hh Hop #Hγ He HΦ /=".
     rewrite low_ctx substitute_expr. iDestruct "Hop" as "(HC1&He2)".
-    wp_bind (substitute _ _). rewrite safe_alt.
-    iApply ("IH" with "[$Hh] [$HC1] [$HΓ] [$He]"). iIntros (?) "_".
-    wp_bind (substitute _ _).
-    iApply (ftlr with "[$Hh] [$HΓ] [$He2]"); first done. iIntros (?) "_".
+    wp_bind (γ _). rewrite safe_alt.
+    iApply ("IH" with "[$Hh] [$HC1] [$Hγ] [$He]"). iIntros (?) "_".
+    wp_bind (γ _).
+    iApply (ftlr with "[$Hh] [$Hγ] [$He2]"). iIntros (?) "_".
     by iApply (wp_low_val_bin_op with "[$HΦ]").
   Qed.
+  Hint Extern 1 (_ ⊢ safe (CBinOpL _ _ _)) => rewrite -safe_bin_op_l.
 
   Lemma safe_bin_op_r op e1 C2 : safe C2 -∗ safe (CBinOpR op e1 C2).
   Proof.
     rewrite (safe_alt (CBinOpR _ _ _)).
-    iIntros "IH". iIntros (Γ p e Φ) "#Hh Hop #HΓ He HΦ /=".
+    iIntros "IH". iIntros (γ p e Φ) "#Hh Hop #Hγ He HΦ /=".
     rewrite low_ctx substitute_expr. iDestruct "Hop" as "(He1&HC2)".
-    wp_bind (substitute _ _).
-    iApply (ftlr with "[$Hh] [$HΓ] [$He1]"); first done. iIntros (?) "_".
-    wp_bind (substitute _ _). rewrite safe_alt.
-    iApply ("IH" with "[$Hh] [$HC2] [$HΓ] [$He]"). iIntros (?) "_".
+    wp_bind (γ _).
+    iApply (ftlr with "[$Hh] [$Hγ] [$He1]"). iIntros (?) "_".
+    wp_bind (γ _). rewrite safe_alt.
+    iApply ("IH" with "[$Hh] [$HC2] [$Hγ] [$He]"). iIntros (?) "_".
     by iApply (wp_low_val_bin_op with "[$HΦ]").
   Qed.
+  Hint Extern 1 (_ ⊢ safe (CBinOpR _ _ _)) => rewrite -safe_bin_op_r.
 
   Lemma safe_if C e1 e2 : safe C -∗ safe (CIf C e1 e2).
   Proof.
     rewrite (safe_alt (CIf _ _ _)).
-    iIntros "IH". iIntros (Γ p e Φ) "#Hh Hif #HΓ He HΦ /=".
+    iIntros "IH". iIntros (γ p e Φ) "#Hh Hif #Hγ He HΦ /=".
     rewrite low_ctx substitute_expr. iDestruct "Hif" as "(HC&He1&He2)".
-    wp_bind (substitute _ _). rewrite safe_alt.
-    iApply ("IH" with "[$Hh] [$HC] [$HΓ] [$He]"). iIntros (?) "_".
+    wp_bind (γ _). rewrite safe_alt.
+    iApply ("IH" with "[$Hh] [$HC] [$Hγ] [$He]"). iIntros (?) "_".
     iApply wp_low_val_if. iNext. iSplit.
-    - by iApply (ftlr with "[$Hh] [$HΓ] [$He1] [$HΦ]").
-    - by iApply (ftlr with "[$Hh] [$HΓ] [$He2] [$HΦ]").
+    - by iApply (ftlr with "[$Hh] [$Hγ] [$He1] [$HΦ]").
+    - by iApply (ftlr with "[$Hh] [$Hγ] [$He2] [$HΦ]").
   Qed.
+  Hint Extern 1 (_ ⊢ safe (CIf _ _ _)) => rewrite -safe_if.
 
   Lemma safe_if_l e0 C1 e2 : safe C1 -∗ safe (CIfL e0 C1 e2).
   Proof.
     rewrite (safe_alt (CIfL _ _ _)).
-    iIntros "IH". iIntros (Γ p e Φ) "#Hh Hif #HΓ He HΦ /=".
+    iIntros "IH". iIntros (γ p e Φ) "#Hh Hif #Hγ He HΦ /=".
     rewrite low_ctx substitute_expr. iDestruct "Hif" as "(He0&HC1&He2)".
-    wp_bind (substitute _ _).
-    iApply (ftlr with "[$Hh] [$HΓ] [$He0]"); first done. iIntros (?) "_".
+    wp_bind (γ _).
+    iApply (ftlr with "[$Hh] [$Hγ] [$He0]"). iIntros (?) "_".
     iApply wp_low_val_if. iNext. iSplit.
-    - rewrite safe_alt. by iApply ("IH" with "[$Hh] [$HC1] [$HΓ] [$He]").
-    - by iApply (ftlr with "[$Hh] [$HΓ] [$He2] [$HΦ]").
+    - rewrite safe_alt. by iApply ("IH" with "[$Hh] [$HC1] [$Hγ] [$He]").
+    - by iApply (ftlr with "[$Hh] [$Hγ] [$He2] [$HΦ]").
   Qed.
+  Hint Extern 1 (_ ⊢ safe (CIfL _ _ _)) => rewrite -safe_if_l.
 
   Lemma safe_if_r e0 e1 C2 : safe C2 -∗ safe (CIfR e0 e1 C2).
   Proof.
     rewrite (safe_alt (CIfR _ _ _)).
-    iIntros "IH". iIntros (Γ p e Φ) "#Hh Hif #HΓ He HΦ /=".
+    iIntros "IH". iIntros (γ p e Φ) "#Hh Hif #Hγ He HΦ /=".
     rewrite low_ctx substitute_expr. iDestruct "Hif" as "(He0&He1&HC2)".
-    wp_bind (substitute _ _).
-    iApply (ftlr with "[$Hh] [$HΓ] [$He0]"); first done. iIntros (?) "_".
+    wp_bind (γ _).
+    iApply (ftlr with "[$Hh] [$Hγ] [$He0]"). iIntros (?) "_".
     iApply wp_low_val_if. iNext. iSplit.
-    - by iApply (ftlr with "[$Hh] [$HΓ] [$He1] [$HΦ]").
-    - rewrite safe_alt. by iApply ("IH" with "[$Hh] [$HC2] [$HΓ] [$He]").
+    - by iApply (ftlr with "[$Hh] [$Hγ] [$He1] [$HΦ]").
+    - rewrite safe_alt. by iApply ("IH" with "[$Hh] [$HC2] [$Hγ] [$He]").
   Qed.
+  Hint Extern 1 (_ ⊢ safe (CIfR _ _ _)) => rewrite -safe_if_r.
 
   Lemma safe_pair_l C1 e2 : safe C1 -∗ safe (CPairL C1 e2).
   Proof.
     rewrite (safe_alt (CPairL _ _)).
-    iIntros "IH". iIntros (Γ p e Φ) "#Hh Hp #HΓ He HΦ /=".
+    iIntros "IH". iIntros (γ p e Φ) "#Hh Hp #Hγ He HΦ /=".
     rewrite low_ctx substitute_expr. iDestruct "Hp" as "(HC1&He2)".
-    wp_bind (substitute _ _). rewrite safe_alt.
-    iApply ("IH" with "[$Hh] [$HC1] [$HΓ] [$He]"). iIntros (v1) "Hv1".
-    wp_bind (substitute _ _).
-    iApply (ftlr with "[$Hh] [$HΓ] [$He2]"); first done. iIntros (v2) "Hv2".
+    wp_bind (γ _). rewrite safe_alt.
+    iApply ("IH" with "[$Hh] [$HC1] [$Hγ] [$He]"). iIntros (v1) "Hv1".
+    wp_bind (γ _).
+    iApply (ftlr with "[$Hh] [$Hγ] [$He2]"). iIntros (v2) "Hv2".
     iApply wp_value; first by rewrite /= (to_of_val v1) (to_of_val v2).
     iApply "HΦ". rewrite (low_val (PairV _ _)). by iFrame.
   Qed.
+  Hint Extern 1 (_ ⊢ safe (CPairL _ _)) => rewrite -safe_pair_l.
 
   Lemma safe_pair_r e1 C2 : safe C2 -∗ safe (CPairR e1 C2).
   Proof.
     rewrite (safe_alt (CPairR _ _)).
-    iIntros "IH". iIntros (Γ p e Φ) "#Hh Hp #HΓ He HΦ /=".
+    iIntros "IH". iIntros (γ p e Φ) "#Hh Hp #Hγ He HΦ /=".
     rewrite low_ctx substitute_expr. iDestruct "Hp" as "(He1&HC2)".
-    wp_bind (substitute _ _).
-    iApply (ftlr with "[$Hh] [$HΓ] [$He1]"); first done. iIntros (v1) "Hv1".
-    wp_bind (substitute _ _). rewrite safe_alt.
-    iApply ("IH" with "[$Hh] [$HC2] [$HΓ] [$He]"). iIntros (v2) "Hv2".
+    wp_bind (γ _).
+    iApply (ftlr with "[$Hh] [$Hγ] [$He1]"). iIntros (v1) "Hv1".
+    wp_bind (γ _). rewrite safe_alt.
+    iApply ("IH" with "[$Hh] [$HC2] [$Hγ] [$He]"). iIntros (v2) "Hv2".
     iApply wp_value; first by rewrite /= (to_of_val v1) (to_of_val v2).
     iApply "HΦ". rewrite (low_val (PairV _ _)). by iFrame.
   Qed.
+  Hint Extern 1 (_ ⊢ safe (CPairR _ _)) => rewrite -safe_pair_r.
 
   Lemma safe_fst C : safe C -∗ safe (CFst C).
   Proof.
     rewrite (safe_alt (CFst _)).
-    iIntros "IH". iIntros (Γ p e Φ) "#Hh HC #HΓ He HΦ /=".
+    iIntros "IH". iIntros (γ p e Φ) "#Hh HC #Hγ He HΦ /=".
     rewrite low_ctx substitute_expr.
-    wp_bind (substitute _ _). rewrite safe_alt.
-    iApply ("IH" with "[$Hh] [$HC] [$HΓ] [$He]"). iIntros (v) "Hv".
+    wp_bind (γ _). rewrite safe_alt.
+    iApply ("IH" with "[$Hh] [$HC] [$Hγ] [$He]"). iIntros (v) "Hv".
     by iApply (wp_low_val_fst with "[$Hv] [$HΦ]").
   Qed.
+  Hint Extern 1 (_ ⊢ safe (CFst _)) => rewrite -safe_fst.
 
   Lemma safe_snd C : safe C -∗ safe (CSnd C).
   Proof.
     rewrite (safe_alt (CSnd _)).
-    iIntros "IH". iIntros (Γ p e Φ) "#Hh HC #HΓ He HΦ /=".
+    iIntros "IH". iIntros (γ p e Φ) "#Hh HC #Hγ He HΦ /=".
     rewrite low_ctx substitute_expr.
-    wp_bind (substitute _ _). rewrite safe_alt.
-    iApply ("IH" with "[$Hh] [$HC] [$HΓ] [$He]"). iIntros (v) "Hv".
+    wp_bind (γ _). rewrite safe_alt.
+    iApply ("IH" with "[$Hh] [$HC] [$Hγ] [$He]"). iIntros (v) "Hv".
     by iApply (wp_low_val_snd with "[$Hv] [$HΦ]").
   Qed.
+  Hint Extern 1 (_ ⊢ safe (CSnd _)) => rewrite -safe_snd.
 
   Lemma safe_inl C : safe C -∗ safe (CInjL C).
   Proof.
     rewrite (safe_alt (CInjL _)).
-    iIntros "IH". iIntros (Γ p e Φ) "#Hh HC #HΓ He HΦ /=".
+    iIntros "IH". iIntros (γ p e Φ) "#Hh HC #Hγ He HΦ /=".
     rewrite low_ctx substitute_expr.
-    wp_bind (substitute _ _). rewrite safe_alt.
-    iApply ("IH" with "[$Hh] [$HC] [$HΓ] [$He]"). iIntros (v) "Hv".
+    wp_bind (γ _). rewrite safe_alt.
+    iApply ("IH" with "[$Hh] [$HC] [$Hγ] [$He]"). iIntros (v) "Hv".
     iApply wp_value; first by rewrite /= (to_of_val v).
     iApply "HΦ". rewrite (low_val (InjLV _)). by iFrame.
   Qed.
+  Hint Extern 1 (_ ⊢ safe (CInjL _)) => rewrite -safe_inl.
 
   Lemma safe_inr C : safe C -∗ safe (CInjR C).
   Proof.
     rewrite (safe_alt (CInjR _)).
-    iIntros "IH". iIntros (Γ p e Φ) "#Hh HC #HΓ He HΦ /=".
+    iIntros "IH". iIntros (γ p e Φ) "#Hh HC #Hγ He HΦ /=".
     rewrite low_ctx substitute_expr.
-    wp_bind (substitute _ _). rewrite safe_alt.
-    iApply ("IH" with "[$Hh] [$HC] [$HΓ] [$He]"). iIntros (v) "Hv".
+    wp_bind (γ _). rewrite safe_alt.
+    iApply ("IH" with "[$Hh] [$HC] [$Hγ] [$He]"). iIntros (v) "Hv".
     iApply wp_value; first by rewrite /= (to_of_val v).
     iApply "HΦ". rewrite (low_val (InjRV _)). by iFrame.
   Qed.
+  Hint Extern 1 (_ ⊢ safe (CInjR _)) => rewrite -safe_inr.
 
   Lemma safe_case C e1 e2 : safe C -∗ safe (CCase C e1 e2).
   Proof.
     rewrite (safe_alt (CCase _ _ _)).
-    iIntros "IH". iIntros (Γ p e Φ) "#Hh Hc #HΓ He HΦ /=".
+    iIntros "IH". iIntros (γ p e Φ) "#Hh Hc #Hγ He HΦ /=".
     rewrite low_ctx substitute_expr. iDestruct "Hc" as "(HC&He1&He2)".
-    wp_bind (substitute _ _). rewrite safe_alt.
-    iApply ("IH" with "[$Hh] [$HC] [$HΓ] [$He]"). iIntros (v) "Hv".
+    wp_bind (γ _). rewrite safe_alt.
+    iApply ("IH" with "[$Hh] [$HC] [$Hγ] [$He]"). iIntros (v) "Hv".
     iApply (wp_low_val_case with "[$Hv]"). iNext. iIntros (v0) "#Hv0".
-    iSplit; wp_bind (substitute _ _).
-    - iApply (ftlr with "[$Hh] [$HΓ] [$He1]"); first done. iIntros (v1) "Hv1".
+    iSplit; wp_bind (γ _).
+    - iApply (ftlr with "[$Hh] [$Hγ] [$He1]"). iIntros (v1) "Hv1".
       by iApply (wp_low_val_app with "[$Hv1 $Hv0] [$HΦ]").
-    - iApply (ftlr with "[$Hh] [$HΓ] [$He2]"); first done. iIntros (v2) "Hv2".
+    - iApply (ftlr with "[$Hh] [$Hγ] [$He2]"). iIntros (v2) "Hv2".
       by iApply (wp_low_val_app with "[$Hv2 $Hv0] [$HΦ]").
   Qed.
+  Hint Extern 1 (_ ⊢ safe (CCase _ _ _)) => rewrite -safe_case.
 
   Lemma safe_case_l e0 C1 e2 : safe C1 -∗ safe (CCaseL e0 C1 e2).
   Proof.
     rewrite (safe_alt (CCaseL _ _ _)).
-    iIntros "IH". iIntros (Γ p e Φ) "#Hh Hc #HΓ He HΦ /=".
+    iIntros "IH". iIntros (γ p e Φ) "#Hh Hc #Hγ He HΦ /=".
     rewrite low_ctx substitute_expr. iDestruct "Hc" as "(He0&HC1&He2)".
-    wp_bind (substitute _ _).
-    iApply (ftlr with "[$Hh] [$HΓ] [$He0]"); first done. iIntros (v) "Hv".
+    wp_bind (γ _).
+    iApply (ftlr with "[$Hh] [$Hγ] [$He0]"). iIntros (v) "Hv".
     iApply (wp_low_val_case with "[$Hv]"). iNext. iIntros (v0) "#Hv0".
-    iSplit; wp_bind (substitute _ _).
+    iSplit; wp_bind (γ _).
     - rewrite safe_alt.
-      iApply ("IH" with "[$Hh] [$HC1] [$HΓ] [$He]"). iIntros (v1) "Hv1".
+      iApply ("IH" with "[$Hh] [$HC1] [$Hγ] [$He]"). iIntros (v1) "Hv1".
       by iApply (wp_low_val_app with "[$Hv1 $Hv0] [$HΦ]").
-    - iApply (ftlr with "[$Hh] [$HΓ] [$He2]"); first done. iIntros (v2) "Hv2".
+    - iApply (ftlr with "[$Hh] [$Hγ] [$He2]"). iIntros (v2) "Hv2".
       by iApply (wp_low_val_app with "[$Hv2 $Hv0] [$HΦ]").
   Qed.
+  Hint Extern 1 (_ ⊢ safe (CCaseL _ _ _)) => rewrite -safe_case_l.
 
   Lemma safe_case_r e0 e1 C2 : safe C2 -∗ safe (CCaseR e0 e1 C2).
   Proof.
     rewrite (safe_alt (CCaseR _ _ _)).
-    iIntros "IH". iIntros (Γ p e Φ) "#Hh Hc #HΓ He HΦ /=".
+    iIntros "IH". iIntros (γ p e Φ) "#Hh Hc #Hγ He HΦ /=".
     rewrite low_ctx substitute_expr. iDestruct "Hc" as "(He0&He1&HC2)".
-    wp_bind (substitute _ _).
-    iApply (ftlr with "[$Hh] [$HΓ] [$He0]"); first done. iIntros (v) "Hv".
+    wp_bind (γ _).
+    iApply (ftlr with "[$Hh] [$Hγ] [$He0]"). iIntros (v) "Hv".
     iApply (wp_low_val_case with "[$Hv]"). iNext. iIntros (v0) "#Hv0".
-    iSplit; wp_bind (substitute _ _).
-    - iApply (ftlr with "[$Hh] [$HΓ] [$He1]"); first done. iIntros (v1) "Hv1".
+    iSplit; wp_bind (γ _).
+    - iApply (ftlr with "[$Hh] [$Hγ] [$He1]"). iIntros (v1) "Hv1".
       by iApply (wp_low_val_app with "[$Hv1 $Hv0] [$HΦ]").
     - rewrite safe_alt.
-      iApply ("IH" with "[$Hh] [$HC2] [$HΓ] [$He]"). iIntros (v2) "Hv2".
+      iApply ("IH" with "[$Hh] [$HC2] [$Hγ] [$He]"). iIntros (v2) "Hv2".
       by iApply (wp_low_val_app with "[$Hv2 $Hv0] [$HΦ]").
   Qed.
+  Hint Extern 1 (_ ⊢ safe (CCaseR _ _ _)) => rewrite -safe_case_r.
 
   Lemma safe_assert C : safe (CAssert C).
-  Proof. iIntros (Γ p e) "_ Hc _ _ /=". rewrite low_ctx. by iExFalso. Qed.
+  Proof. iIntros (γ p e) "_ Hc _ _ /=". rewrite low_ctx. by iExFalso. Qed.
+  Hint Extern 1 (_ ⊢ safe (CAssert _)) => rewrite -safe_assert.
 
   Lemma safe_fork C : safe C -∗ safe (CFork C).
   Proof.
     rewrite (safe_alt (CFork _)).
-    iIntros "IH". iIntros (Γ p e Φ) "#Hh HC #HΓ He HΦ /=".
+    iIntros "IH". iIntros (γ p e Φ) "#Hh HC #Hγ He HΦ /=".
     rewrite low_ctx substitute_expr. iApply wp_fork. iNext. iSplitL "HΦ".
     - iApply "HΦ". by rewrite low_val low_lit.
-    - rewrite safe_alt. iApply ("IH" with "[$Hh] [$HC] [$HΓ] [$He]").
+    - rewrite safe_alt. iApply ("IH" with "[$Hh] [$HC] [$Hγ] [$He]").
       by iIntros.
   Qed.
+  Hint Extern 1 (_ ⊢ safe (CFork _)) => rewrite -safe_fork.
 
   Lemma safe_alloc C : safe C -∗ safe (CAlloc C).
   Proof.
     rewrite (safe_alt (CAlloc _)).
-    iIntros "IH". iIntros (Γ p e Φ) "#Hh HC #HΓ He HΦ /=".
+    iIntros "IH". iIntros (γ p e Φ) "#Hh HC #Hγ He HΦ /=".
     rewrite low_ctx substitute_expr.
-    wp_bind (substitute _ _). rewrite safe_alt.
-    iApply ("IH" with "[$Hh] [$HC] [$HΓ] [$He]"). iIntros (v) "Hv".
+    wp_bind (γ _). rewrite safe_alt.
+    iApply ("IH" with "[$Hh] [$HC] [$Hγ] [$He]"). iIntros (v) "Hv".
     iApply (wp_alloc_low with "[$Hh $Hv]"); [by rewrite to_of_val|done|].
     iNext. iIntros (l) "#Hl". iApply "HΦ". by rewrite low_val low_lit.
   Qed.
+  Hint Extern 1 (_ ⊢ safe (CAlloc _)) => rewrite -safe_alloc.
 
   Lemma safe_load C : safe C -∗ safe (CLoad C).
   Proof.
     rewrite (safe_alt (CLoad _)).
-    iIntros "IH". iIntros (Γ p e Φ) "#Hh HC #HΓ He HΦ /=".
+    iIntros "IH". iIntros (γ p e Φ) "#Hh HC #Hγ He HΦ /=".
     rewrite low_ctx substitute_expr.
-    wp_bind (substitute _ _). rewrite safe_alt.
-    iApply ("IH" with "[$Hh] [$HC] [$HΓ] [$He]"). iIntros (v) "Hv".
+    wp_bind (γ _). rewrite safe_alt.
+    iApply ("IH" with "[$Hh] [$HC] [$Hγ] [$He]"). iIntros (v) "Hv".
     by iApply (wp_low_val_load with "[$Hh $Hv] [$HΦ]").
   Qed.
+  Hint Extern 1 (_ ⊢ safe (CLoad _)) => rewrite -safe_load.
 
   Lemma safe_store_l C1 e2 : safe C1 -∗ safe (CStoreL C1 e2).
   Proof.
     rewrite (safe_alt (CStoreL _ _)).
-    iIntros "IH". iIntros (Γ p e Φ) "#Hh Hp #HΓ He HΦ /=".
+    iIntros "IH". iIntros (γ p e Φ) "#Hh Hp #Hγ He HΦ /=".
     rewrite low_ctx substitute_expr. iDestruct "Hp" as "(HC1&He2)".
-    wp_bind (substitute _ _). rewrite safe_alt.
-    iApply ("IH" with "[$Hh] [$HC1] [$HΓ] [$He]"). iIntros (v1) "Hv1".
-    wp_bind (substitute _ _).
-    iApply (ftlr with "[$Hh] [$HΓ] [$He2]"); first done. iIntros (v2) "Hv2".
+    wp_bind (γ _). rewrite safe_alt.
+    iApply ("IH" with "[$Hh] [$HC1] [$Hγ] [$He]"). iIntros (v1) "Hv1".
+    wp_bind (γ _).
+    iApply (ftlr with "[$Hh] [$Hγ] [$He2]"). iIntros (v2) "Hv2".
     by iApply (wp_low_val_store with "[$Hh $Hv1 $Hv2] [$HΦ]").
   Qed.
+  Hint Extern 1 (_ ⊢ safe (CStoreL _ _)) => rewrite -safe_store_l.
 
   Lemma safe_store_r e1 C2 : safe C2 -∗ safe (CStoreR e1 C2).
   Proof.
     rewrite (safe_alt (CStoreR _ _)).
-    iIntros "IH". iIntros (Γ p e Φ) "#Hh Hp #HΓ He HΦ /=".
+    iIntros "IH". iIntros (γ p e Φ) "#Hh Hp #Hγ He HΦ /=".
     rewrite low_ctx substitute_expr. iDestruct "Hp" as "(He1&HC2)".
-    wp_bind (substitute _ _).
-    iApply (ftlr with "[$Hh] [$HΓ] [$He1]"); first done. iIntros (v1) "Hv1".
-    wp_bind (substitute _ _). rewrite safe_alt.
-    iApply ("IH" with "[$Hh] [$HC2] [$HΓ] [$He]"). iIntros (v2) "Hv2".
+    wp_bind (γ _).
+    iApply (ftlr with "[$Hh] [$Hγ] [$He1]"). iIntros (v1) "Hv1".
+    wp_bind (γ _). rewrite safe_alt.
+    iApply ("IH" with "[$Hh] [$HC2] [$Hγ] [$He]"). iIntros (v2) "Hv2".
     by iApply (wp_low_val_store with "[$Hh $Hv1 $Hv2] [$HΦ]").
   Qed.
+  Hint Extern 1 (_ ⊢ safe (CStoreR _ _)) => rewrite -safe_store_r.
 
   Lemma safe_cas_l C e1 e2 : safe C -∗ safe (CCASL C e1 e2).
   Proof.
     rewrite (safe_alt (CCASL _ _ _)).
-    iIntros "IH". iIntros (Γ p e Φ) "#Hh Hc #HΓ He HΦ /=".
+    iIntros "IH". iIntros (γ p e Φ) "#Hh Hc #Hγ He HΦ /=".
     rewrite low_ctx substitute_expr. iDestruct "Hc" as "(HC&He1&He2)".
-    wp_bind (substitute _ _). rewrite safe_alt.
-    iApply ("IH" with "[$Hh] [$HC] [$HΓ] [$He]"). iIntros (v0) "Hv0".
-    wp_bind (substitute _ _).
-    iApply (ftlr with "[$Hh] [$HΓ] [$He1]"); first done. iIntros (v1) "_".
-    wp_bind (substitute _ _).
-    iApply (ftlr with "[$Hh] [$HΓ] [$He2]"); first done. iIntros (v2) "Hv2".
+    wp_bind (γ _). rewrite safe_alt.
+    iApply ("IH" with "[$Hh] [$HC] [$Hγ] [$He]"). iIntros (v0) "Hv0".
+    wp_bind (γ _).
+    iApply (ftlr with "[$Hh] [$Hγ] [$He1]"). iIntros (v1) "_".
+    wp_bind (γ _).
+    iApply (ftlr with "[$Hh] [$Hγ] [$He2]"). iIntros (v2) "Hv2".
     by iApply (wp_low_val_cas with "[$Hh $Hv0 $Hv2] [$HΦ]").
   Qed.
+  Hint Extern 1 (_ ⊢ safe (CCASL _ _ _)) => rewrite -safe_cas_l.
 
   Lemma safe_cas_m e0 C1 e2 : safe C1 -∗ safe (CCASM e0 C1 e2).
   Proof.
     rewrite (safe_alt (CCASM _ _ _)).
-    iIntros "IH". iIntros (Γ p e Φ) "#Hh Hc #HΓ He HΦ /=".
+    iIntros "IH". iIntros (γ p e Φ) "#Hh Hc #Hγ He HΦ /=".
     rewrite low_ctx substitute_expr. iDestruct "Hc" as "(He0&HC1&He2)".
-    wp_bind (substitute _ _).
-    iApply (ftlr with "[$Hh] [$HΓ] [$He0]"); first done. iIntros (v0) "Hv0".
-    wp_bind (substitute _ _). rewrite safe_alt.
-    iApply ("IH" with "[$Hh] [$HC1] [$HΓ] [$He]"). iIntros (v1) "Hv1".
-    wp_bind (substitute _ _).
-    iApply (ftlr with "[$Hh] [$HΓ] [$He2]"); first done. iIntros (v2) "Hv2".
+    wp_bind (γ _).
+    iApply (ftlr with "[$Hh] [$Hγ] [$He0]"). iIntros (v0) "Hv0".
+    wp_bind (γ _). rewrite safe_alt.
+    iApply ("IH" with "[$Hh] [$HC1] [$Hγ] [$He]"). iIntros (v1) "Hv1".
+    wp_bind (γ _).
+    iApply (ftlr with "[$Hh] [$Hγ] [$He2]"). iIntros (v2) "Hv2".
     by iApply (wp_low_val_cas with "[$Hh $Hv0 $Hv2] [$HΦ]").
   Qed.
+  Hint Extern 1 (_ ⊢ safe (CCASM _ _ _)) => rewrite -safe_cas_m.
 
   Lemma safe_cas_r e0 e1 C2 : safe C2 -∗ safe (CCASR e0 e1 C2).
   Proof.
     rewrite (safe_alt (CCASR _ _ _)).
-    iIntros "IH". iIntros (Γ p e Φ) "#Hh Hc #HΓ He HΦ /=".
+    iIntros "IH". iIntros (γ p e Φ) "#Hh Hc #Hγ He HΦ /=".
     rewrite low_ctx substitute_expr. iDestruct "Hc" as "(He0&He1&HC2)".
-    wp_bind (substitute _ _).
-    iApply (ftlr with "[$Hh] [$HΓ] [$He0]"); first done. iIntros (v0) "Hv0".
-    wp_bind (substitute _ _).
-    iApply (ftlr with "[$Hh] [$HΓ] [$He1]"); first done. iIntros (v1) "_".
-    wp_bind (substitute _ _). rewrite safe_alt.
-    iApply ("IH" with "[$Hh] [$HC2] [$HΓ] [$He]"). iIntros (v2) "Hv2".
+    wp_bind (γ _).
+    iApply (ftlr with "[$Hh] [$Hγ] [$He0]"). iIntros (v0) "Hv0".
+    wp_bind (γ _).
+    iApply (ftlr with "[$Hh] [$Hγ] [$He1]"). iIntros (v1) "_".
+    wp_bind (γ _). rewrite safe_alt.
+    iApply ("IH" with "[$Hh] [$HC2] [$Hγ] [$He]"). iIntros (v2) "Hv2".
     by iApply (wp_low_val_cas with "[$Hh $Hv0 $Hv2] [$HΦ]").
   Qed.
+  Hint Extern 1 (_ ⊢ safe (CCASR _ _ _)) => rewrite -safe_cas_r.
 
-  Theorem robust_safety' C : safe C.
-  Proof.
-    iStartProof.
-    iInduction C as [| | | | | | | | | | | | | | | | | | | | | | | | | | |] "IH".
-    - by rewrite -safe_hole.
-    - by rewrite -safe_rec.
-    - by rewrite -safe_app_l.
-    - by rewrite -safe_app_r.
-    - by rewrite -safe_un_op.
-    - by rewrite -safe_bin_op_l.
-    - by rewrite -safe_bin_op_r.
-    - by rewrite -safe_if.
-    - by rewrite -safe_if_l.
-    - by rewrite -safe_if_r.
-    - by rewrite -safe_pair_l.
-    - by rewrite -safe_pair_r.
-    - by rewrite -safe_fst.
-    - by rewrite -safe_snd.
-    - by rewrite -safe_inl.
-    - by rewrite -safe_inr.
-    - by rewrite -safe_case.
-    - by rewrite -safe_case_l.
-    - by rewrite -safe_case_r.
-    - by rewrite -safe_assert.
-    - by rewrite -safe_fork.
-    - by rewrite -safe_alloc.
-    - by rewrite -safe_load.
-    - by rewrite -safe_store_l.
-    - by rewrite -safe_store_r.
-    - by rewrite -safe_cas_l.
-    - by rewrite -safe_cas_m.
-    - by rewrite -safe_cas_r.
-  Qed.
+  Hint Extern 2 =>
+    match goal with
+    | IH : True ⊢ safe ?C |- True ⊢ safe (_ ?C) => rewrite IH
+    end.
+
+  Theorem robust_safetyI' C : safe C.
+  Proof. rewrite/uPred_valid. by induction C; auto. Qed.
 
   (** The internal version of [robust_safety]. *)
-  Corollary robust_safetyI C Γ p e Φ `{!Closed [] e} :
-    heap_ctx -∗ low C -∗ low Γ -∗ □ WP e @ p; ⊤ {{ low }} -∗
-    (∀ v, low v -∗ Φ v) -∗ WP substitute Γ (ctx_fill C e) ?{{ Φ }}.
+  Corollary robust_safetyI C γ p e Φ `{!Closed [] e} :
+    heap_ctx -∗ low C -∗ low γ -∗ □ WP e @ p; ⊤ {{ low }} -∗
+    (∀ v, low v -∗ Φ v) -∗ WP γ (ctx_fill C e) ?{{ Φ }}.
   Proof.
-    iIntros "Hh HC HΓ #He". rewrite -wp_wand.
-    iApply (robust_safety' with "[$Hh] [$HC] [$HΓ]"). by iAlways; iSplit.
+    iIntros "Hh HC Hγ #He". rewrite -wp_wand.
+    iApply (robust_safetyI' with "[$Hh] [$HC] [$Hγ]"). by iAlways; iSplit.
   Qed.
 End robust_safety.
